src/PermHashmap.v
@@ -16,14 +16,14 @@ Definition hash2 sz1 sz2 (a : word sz1) (b : word sz2) :=
     When the list of values is empty, h must be equal to the default hash
     value.
 *)
-Inductive hash_list_rep : (list tagged_block) -> word hashlen -> hashmap -> Prop :=
+Inductive hash_list_rep : (list valu) -> word hashlen -> hashmap -> Prop :=
   | HL_nil : forall hl hm,
       hl = default_hash ->
       hash_list_rep nil hl hm
   | HL_cons : forall l hl hl' x hm,
       hash_list_rep l hl hm ->
-      hl' = hash2 (encode x) hl ->
-      hashmap_get hm hl' = Some (existT _ _ (Word.combine (encode x) hl)) ->
+      hl' = hash2 x hl ->
+      hashmap_get hm hl' = Some (existT _ _ (Word.combine x hl)) ->
       hash_list_rep (x :: l) hl' hm.
 
 (** hash_list_prefixes takes in a list of values vl, a list of hashes hl,
@@ -32,7 +32,7 @@ Inductive hash_list_rep : (list tagged_block) -> word hashlen -> hashmap -> Prop
     TODO: This could probably be merged into hash_list_rep, but not sure
     how much more work that would be right now.
 *)
-Inductive hash_list_prefixes : list tagged_block -> list (word hashlen) -> hashmap -> Prop :=
+Inductive hash_list_prefixes : list valu -> list (word hashlen) -> hashmap -> Prop :=
   | HLP_default : forall hm,
     hash_list_prefixes nil nil hm
   | HLP_cons : forall v h vl hl hm,
@@ -72,7 +72,7 @@ Ltac contradict_hashmap_get_default H hm :=
   let Hx := fresh in
   contradict H;
   destruct hm; unfold hashmap_get, default_hash;
-  destruct (weq (hash_fwd (encode tagged_block0)) (hash_fwd (encode tagged_block0)));
+  destruct (weq (hash_fwd default_valu) (hash_fwd default_valu));
   intro Hx; try existT_wordsz_neq Hx;
   intuition.
 
@@ -90,7 +90,7 @@ Proof.
 Qed.
 
 Theorem hashmap_get_default : forall hm,
-  hashmap_get hm default_hash = Some (existT _ _ default_encoding).
+  hashmap_get hm default_hash = Some (existT _ _ default_valu).
 Proof.
   unfold hashmap_get.
   destruct hm; destruct (weq default_hash default_hash);
@@ -162,7 +162,6 @@ Proof.
   inversion H10.
   existT_wordsz_eq H2.
   intuition.
-  apply encode_inj in H4.
   subst; apply IHl1 in H8; try congruence.  
 Qed.
 
@@ -272,7 +271,7 @@ Qed.
 Lemma hash_list_prefixes_forall : forall i vl hl hm default defaultv,
   hash_list_prefixes vl hl hm ->
   i < length hl - 1 ->
-  selN hl i default = hash2 (encode (selN vl i defaultv)) (selN hl (i + 1) default).
+  selN hl i default = hash2 (selN vl i defaultv) (selN hl (i + 1) default).
 Proof.
   induction i; intros.
   destruct hl. inversion H0.
